Prove Bitmap.Set

lib/Bitmap.dfy
@@ -4,34 +4,6 @@ include "NativeTypes.s.dfy"
 module Bitmap {
   import opened NativeTypes
 
-  predicate {:opaque} BitsSetAtIB(bitsSeq: seq<bv64>, i: nat, b: nat)
-  requires i < |bitsSeq|
-  requires b < 64
-  {
-    && bitsSeq[i] & (1 << b) != 0
-  }
-
-  predicate {:opaque} BitsSetAtC(bitsSeq: seq<bv64>, c: nat)
-  requires c / 64 < |bitsSeq|
-  {
-    && BitsSetAtIB(bitsSeq, c / 64, c % 64)
-  }
-
-  predicate ITimes64WithinUint64(i: nat)
-  {
-    && i * 64 < 0x1_0000_0000_0000_0000
-  }
-
-  predicate {:opaque} BitsMatchesContents(bitsSeq: seq<bv64>, contents: set<uint64>)
-  {
-    && (forall c: nat | c < 0x1_0000_0000_0000_0000 && (c as uint64) in contents && c / 64 < |bitsSeq| :: BitsSetAtC(bitsSeq, c))
-  }
-
-  predicate {:opaque} ContentsMatchesBits(bitsSeq: seq<bv64>, contents: set<uint64>)
-  {
-    && (forall i: nat, b: nat | i < |bitsSeq| && ITimes64WithinUint64(i) && b < 64 && BitsSetAtIB(bitsSeq, i, b) ::
-        (((i * 64) + b) as uint64) in contents)
-  }
 
   class Bitmap {
     var bits: array<bv64>;
@@ -39,12 +11,46 @@ module Bitmap {
     ghost var Contents: set<uint64>;
     ghost var Repr: set<object>;
 
+    static predicate BitBSet(word: bv64, b: nat)
+    requires b < 64
+    {
+      && word & (1 << b) != 0
+    }
+
+    static predicate BitsSetAtIB(bitsSeq: seq<bv64>, i: nat, b: nat)
+    requires i < |bitsSeq|
+    requires b < 64
+    {
+      && BitBSet(bitsSeq[i], b)
+    }
+
+    static predicate BitsSetAtC(bitsSeq: seq<bv64>, c: nat)
+    requires c / 64 < |bitsSeq|
+    {
+      && BitsSetAtIB(bitsSeq, c / 64, c % 64)
+    }
+
+    static predicate ITimes64WithinUint64(i: nat)
+    {
+      && i * 64 < 0x1_0000_0000_0000_0000
+    }
+
+    static predicate {:opaque} BitsMatchesContents(bitsSeq: seq<bv64>, contents: set<uint64>)
+    {
+      && (forall c: nat | c < 0x1_0000_0000_0000_0000 && (c as uint64) in contents && c / 64 < |bitsSeq| :: BitsSetAtC(bitsSeq, c))
+    }
+
+    static predicate {:opaque} ContentsMatchesBits(bitsSeq: seq<bv64>, contents: set<uint64>)
+    {
+      && (forall i: nat, b: nat | i < |bitsSeq| && ITimes64WithinUint64(i) && b < 64 && BitsSetAtIB(bitsSeq, i, b) ::
+          (((i * 64) + b) as uint64) in contents)
+    }
+
     predicate ReprInv()
     reads this, this.Repr
     {
       && this.Repr == { this, this.bits }
     }
-
 
     protected predicate Inv()
     ensures Inv() ==> ReprInv()
@@ -70,10 +76,20 @@ module Bitmap {
       Contents := {};
       Repr := { this, this.bits };
 
-      assume false;
+      reveal_BitsMatchesContents();
+      reveal_ContentsMatchesBits();
+    }
 
-      // reveal_BitsMatchesContents();
-      // reveal_ContentsMatchesBits();
+    static lemma SetABit(before: seq<bv64>, after: seq<bv64>, i: nat, b: nat)
+    requires |after| == |before|
+    requires i < |before|
+    requires b < 64
+    requires forall i': nat | i' < |before| && i' != i :: after[i'] == before[i']
+    requires after[i] == before[i] | (1 << b)
+    ensures BitBSet(after[i], b as nat)
+    ensures forall b': nat | b' != b as nat && b' < 64 :: BitBSet(before[i], b') <==> BitBSet(after[i], b')
+    {
+      assume false;
     }
 
     method Set(c: uint64)
@@ -84,21 +100,53 @@ module Bitmap {
     ensures this.Repr == old(this.Repr)
     modifies this, this.Repr
     {
-      this.bits[c / 64] := this.bits[c / 64] | (1 << (c % 64));
+      var i: uint64 := c / 64;
+      var b: uint64 := c % 64;
+
+      this.bits[i] := this.bits[i] | (1 << b);
+      SetABit(old(this.bits[..]), this.bits[..], i as nat, b as nat);
+      assert BitBSet(this.bits[i], b as nat);
+      assert forall b': nat | b' != b as nat && b' < 64 :: BitBSet(bits[i], b') <==> old(BitBSet(bits[i], b'));
 
       Contents := Contents + {c};
 
-      forall c: nat | c < 0x1_0000_0000_0000_0000 && (c as uint64) in Contents && c / 64 < bits.Length
-      ensures BitsSetAtC(bits[..], c) {
-        assume false;
+      forall c': nat | c' < 0x1_0000_0000_0000_0000 && (c' as uint64) in Contents && c' / 64 < bits.Length
+      ensures BitsSetAtC(bits[..], c') {
+        var i' := c' / 64;
+        var b' := c' % 64;
+        if i' == i as nat {
+          if b' == b as nat {
+          } else {
+            reveal_BitsMatchesContents();
+            assert BitsSetAtC(old(bits[..]), c'); // observe
+            assert BitsSetAtIB(old(bits[..]), i', b'); // observe
+            assert old(BitBSet(bits[i'], b')); // observe
+            assert BitBSet(bits[i], b'); // observe
+            assert BitsSetAtIB(bits[..], i', b'); // observe
+          }
+        } else {
+          reveal_BitsMatchesContents();
+          assert BitsSetAtC(old(bits[..]), c');
+          /* (doc) assert this.bits[c' / 64] == old(this.bits[c' / 64]); */
+        }
       }
-      forall i: nat, b: nat | i < bits.Length && ITimes64WithinUint64(i) && b < 64 && BitsSetAtIB(bits[..], i, b)
-      ensures (((i * 64) + b) as uint64) in Contents
+      forall i': nat, b': nat | i' < bits.Length && ITimes64WithinUint64(i') && b' < 64 && BitsSetAtIB(bits[..], i', b')
+      ensures (((i' * 64) + b') as uint64) in Contents
       {
-        assume false;
+        var c' := (i' * 64) + b';
+        if i' == i as nat {
+          if b' == b as nat {
+          } else {
+            reveal_ContentsMatchesBits();
+            assert old(BitsSetAtIB(bits[..], i', b')); // observe
+          }
+        } else {
+          reveal_ContentsMatchesBits();
+          assert old(BitsSetAtIB(bits[..], i', b')); // observe
+        }
       }
-      // reveal_BitsMatchesContents();
-      // reveal_ContentsMatchesBits();
+      reveal_BitsMatchesContents();
+      reveal_ContentsMatchesBits();
       assert Inv();
     }
 
